proof/correctness/for.ec
@@ -1,0 +1,97 @@
+require import AllCore StdOrder IntMin IntDiv.
+
+import IntOrder.
+
+abstract theory FOR.
+
+  type t, it, ct.
+
+  op incr : it -> t -> t.
+  op cond : ct -> t -> bool.
+  op out : it -> ct -> t -> int.
+  op finite : it -> ct -> t -> bool.
+  op val : it -> t -> int -> t.
+
+  abbrev ncond_val i c x n = ! cond c (val i x n).
+  abbrev form i c x n = (0 <= n <= out i c x).
+  op inv i c x v = exists n , (v = (val i x n)) /\ (form i c x n).
+
+  axiom val_iter i x n : 0 <= n => val i x n = (iter n (incr i) x).
+  axiom finite_nsempty i c x : finite i c x => ! sempty (pcap (ncond_val i c x)).
+  axiom pmin_out i c x : finite i c x => pmin (ncond_val i c x) = out i c x.
+
+  lemma inv_loop i c x v : finite i c x => inv i c x v => cond c v => inv i c x (incr i v).
+  proof.
+    move => Hfin [n [->> [le0n /ler_eqVlt lenout]]] Hcond.
+    case lenout => [->>|ltnout].
+    + by have:= pmin_mem _ (finite_nsempty _ _ _ Hfin); rewrite (pmin_out _ _ _ Hfin) /= => /negP Hncond; have:= (Hncond Hcond).
+    exists (n+1); do!split.
+    + by rewrite !val_iter ?addr_ge0 // iterS.
+    + by apply addr_ge0.
+    by move => _; apply ltzE.
+  qed.
+
+  lemma inv_in i c x : finite i c x => inv i c x x.
+  proof.
+    move => Hfin; exists 0; rewrite val_iter // iter0 //=.
+    rewrite -(pmin_out _ _ _ Hfin).
+    by apply ge0_pmin.
+  qed.
+
+  lemma inv_out i c x v : finite i c x => inv i c x v => !(cond c v) => v = (val i x (out i c x)).
+  proof.
+    move => Hfin [n [->> [le0n /ler_eqVlt lenout]]] Hncond.
+    case lenout => [-> //|ltnout].
+    have:= (pmin_min _ _ (finite_nsempty _ _ _ Hfin) le0n Hncond).
+    by rewrite (pmin_out _ _ _ Hfin) => /lezNgt /negP nltnout; move: (nltnout ltnout).
+  qed.
+
+end FOR.
+
+
+
+theory FOR_INT_ADD_LT.
+
+  clone include FOR with 
+    type t <- int,
+    type it <- int,
+    type ct <- int,
+    op incr <- (fun i x : int => x + i),
+    op cond <- (fun c x : int => x < c),
+    op out = (fun i c x : int => max (- (x - c) %/ i) 0),
+    op finite <- (fun i c x : int => (0 < i)),
+    op val <- (fun i x n : int => x + n * i)
+    proof *.
+
+    realize val_iter.
+    proof.
+      by move => i x; elim; [rewrite iter0|move => n le0n; rewrite mulzDl addzA iterS // => <- /=].
+    qed.
+
+    realize finite_nsempty.
+    proof.
+      move => i c x lt0i; apply semptyNP.
+      exists (out i c x); rewrite /out maxrE.
+      case: (0 <= - (x - c) %/ i) => [le0_|/ltzNge lt_0]; split => //=.
+      + apply/negP => /ltr_subr_addl; rewrite mulNr => /ltr_oppl; rewrite opprB /=.
+        by apply /ler_gtF; apply lez_floor; apply gtr_eqF.
+      move: lt_0 => /ltr_oppl /= lt0_; apply/ltr_gtF/subr_gt0.
+      by apply (ltr_le_trans ((x - c) %/ i * i)); [apply mulr_gt0|apply/lez_floor/gtr_eqF].
+    qed.
+
+    (*TODO: use new lemmas on pmin.*)
+    realize pmin_out.
+    proof.
+      move => i c x lt0i.
+      admit.
+    qed.
+
+end FOR_INT_ADD_LT.
+
+
+
+(*TODO: an int logarithm or something for a FOR_INT_DIV_GE ?*)
+
+require import RealExp.
+
+search _ ilog.
